added compact printing in the SquiggleEq library.
used it to define compact (not necessarily pretty) printing for L4a.
(also updated SquiggleEq to the latest version fef0f1dfacc6b636a129558ee8e9836eb77476f1)
Although it produces decent results on simple examples, it
runs into stack overflow when printing Gcd (compiled to L4a).

Also, Quoting Gcd is very slow -- takes almost a minute.
In contrast, Extraction is very fast on Gcd.

libraries/SquiggleEq/varImplPeano.v
@@ -31,9 +31,9 @@ Require Import Coq.Lists.List.
 Import ListNotations.
 
 Section PeanoVarInstance.
-Context (VarClass :Type) {Hd : Deq VarClass}.
+Context (VarCl :Type) {Hd : Deq VarCl}.
 
-Notation VType := ((nat * VarClass)%type).
+Notation VType := ((nat * VarCl)%type).
 
 (*Instance DeqVType : Deq VType.
   unfold VType. eauto with typeclass_instances.
@@ -44,26 +44,31 @@ Require Import Omega.
 Require Import Coq.Sorting.Sorting.
 Print VarType.
 
-Variable defClass : VarClass.
+Variable defClass : VarCl.
 
-Definition freshVarsPeano (n:nat) (oc : option VarClass) (avoid original : list VType) : list VType :=  
+Global Instance freshVarsPeano : FreshVars VType VarCl :=
+fun (n:nat) (oc : option VarCl) (avoid original : list VType) =>
 let c := match oc with | Some x => x | None => defClass end in
 let maxn := maxl (map fst avoid) in
 List.map (fun x => (x,c)) (seq (S maxn) n).
 
+Global Instance varClassPeano : VarClass VType VarCl := snd.
+
+
 Require Import LibTactics.
 Require Import tactics.
 
-Global Instance VarTypePeano : VarType VType VarClass.
-  apply Build_VarType with (varClass:=snd) (freshVars := freshVarsPeano).
+Global Instance VarTypePeano : VarType VType VarCl.
+  apply Build_VarType.
   intros.
   subst lf. unfold freshVarsPeano.
   autorewrite with list.
   split;[split|].
-- apply NoDup_map_inv with (f:=fst). rewrite map_map.
+- apply NoDup_map_inv with (f:=fst). setoid_rewrite map_map.
   simpl. rewrite map_id. apply seq_NoDup.
-- split; [| refl].
-  intros ? Hin.
+- setoid_rewrite map_length. rewrite seq_length.
+  split; [| refl].
+  intros ? Hin. unfold freshVars in Hin.
   rewrite in_map_iff in Hin.
   setoid_rewrite in_seq in Hin.
   exrepnd. inverts Hin1.
@@ -72,7 +77,7 @@ Global Instance VarTypePeano : VarType VType VarClass.
   simpl in Hinc.
   apply maxl_prop in Hinc.
   omega.
-- introv ? Hin. subst.
+- introv ? Hin. subst. unfold freshVars in Hin.
   apply in_map_iff in Hin.
   exrepnd. cpx.
 Defined.
